Let $\tm \in \termsdist$ be a correct term,
and $\tctx \vdash \tm : \typ$ its (unique) type derivation.
Let $\var$ be any variable,
and consider the $n \geq 0$ free occurrences of the variable $\var$ in the term $\tm$,
more precisely, write $\tm$ as $\tm = \conhat\of{\var^{\typ_1},\hdots,\var^{\typ_n}}$,
where $\conhat$ is a context with $n$-holes such that $\var \not\in \fv{\conhat}$.
We will prove that $\tctx(\var) = \set{\typ_1,\hdots,\typ_n}$.

\begin{proof}
By induction on $\tm$.
\begin{enumerate}
\item \Case{Variable (same), $\tm = \var^\typ$}
  By uniqueness of derivations, we have that $\set{\var : \set{\typ}} \vdash \var^\typ : \typ$.
  Also, $\conhat = \conbase$ and $\tm = \conhat\of{\var^\typtwo}$.
  And we also have that $\tctx(\var) = \set{\typ}$, so we are done.
\item \Case{Variable (different), $\tm = \vartwo^\typ$}
  By uniqueness of derivations, we have that $\set{\vartwo : \set{\typ}} \vdash \vartwo^\typ : \typ$.
  Also, $\conhat = \vartwo^\typ$ (that is, $\conhat$ does not have any holes) and $\tm = \conhat$.
  And we also have that $\tctx(\var) = \emptyset$, so we are done.
\item \Case{Abstraction, $\tm = \lam{\vartwo}{\tmthree}$}
  By uniqueness of derivations, we have that the derivation of $\tm$ is the following.
    \[
      \indrule{\toI}{
        \tctx \oplus \vartwo : \lsetenum{\typthree}{1}{n} \vdash \tmthree : \typ_1
      }{
        \tctx \vdash \lamp{\lab}{\vartwo}{\tmthree} : \lsetenum{\typthree}{1}{n} \tolab{\lab} \typ_1
      }
    \]
  Given that $\tmthree$ is a subterm of $\tm$, it is correct. So we may use the inductive hypothesis,
    which tells us that there is a context $\conhat_1$
    such that $\tmthree = \conhat_1\of{\var^{\typ_1},\hdots,\var^{\typ_n}}$
    (where $\var \not\in \fv\conhat$) and
    $(\tctx \oplus \vartwo : \lsetenum{\typthree}{1}{n})(\var) = \set{\typ_1,\hdots,\typ_n}$.

  Then, we take $\conhat$ to be $\lamp{\lab}{\vartwo}{\conhat_1}$.
    Note that $\var \not\in \fv\conhat$, and also that
    $\tctx(\var) = (\tctx \oplus \vartwo : \lsetenum{\typthree}{1}{n})(\var) = \set{\typ_1,\hdots,\typ_n}$.
\item \Case{Application, $\tm = \tmthree [\tmfour_1,\hdots,\tmfour_n]$}
  By uniqueness of derivations, we have that the derivation of $\tm$ is the following.
    \[
      \indrule{\toE}{
        \tctx_0 \vdash \tmthree : \lset{\typtwo_1,\hdots,\typtwo_n} \tolab{\lab} \typ
        \HS
        \left( \tctx_i \vdash \tmfour_i : \typtwo_i \right)_{i=1}^{n}
      }{
        \tctx = \tctx_0 +_{i=1}^{n} \tctx_i \vdash \tmthree \lsetenum{\tmfour}{1}{n} : \typ
      }
    \]
  Given that $\tmthree$ and all $\tmfour_i$ are subterms of $\tm$, they are correct;
    so can use inductive hypothesis on them.
  By inductive hypothesis on $\tmthree$,
    we get that $\tmthree = \conhat_0\of{\var^{\typ_{0,0}},\hdots,\var^{\typ_{0,m_0}}}$
  (where $\var \not\in \fv{\conhat_0}$) and $\tctx_0(\var) = \set{\typ_{0,0},\hdots,\typ_{0,m_0}}$.
  On the other hand, by inductive hypothesis on $\tmfour_i$,
    we get that $\tmfour_i = \conhat_i\of{\var^{\typ_{i,0}},\hdots,\var^{\typ_{i, m_i}}}$
  (where $\var \not\in \fv{\conhat_i}$) and $\tctx_i(\var) = \set{\typ_{i,0},\hdots,\typ_{i,m_i}}$.

  If we take $\conhat$ to be $\conhat_0 \lset{\conhat_1, \hdots, \conhat_n}$, we have that
    $\var \not\in \fv\conhat$ and
    \begin{equation*}\begin{split}
      \tm
     & = \tmthree [\tmfour_1, \hdots, \tmfour_n] \\
     & = \conhat_0\of{\var^{\typ_{0,0}},\hdots,\var^{\typ_{0,n_0}}}
         [\conhat_1\of{\var^{\typ_{1,0}},\hdots,\var^{\typ_{1,m_1}}},\hdots
          \conhat_n\of{\var^{\typ_{n,0}},\hdots,\var^{\typ_{n,m_n}}}] \\
     & = (\conhat_0 \lset{\conhat_1, \hdots, \conhat_n})\of{\var^{\typ_{0,0}},\hdots,
        \var^{\typ_{0,n_0}}, \hdots, \var^{\typ_{n,0}},\hdots,\var^{\typ_{n,m_n}}} \\
    \end{split}\end{equation*}
  To end the proof, we check the condition on the context.
    \begin{equation*}\begin{split}
      \tctx(\var)
        & = (\tctx_0 +_{i=1}^{n} \tctx_i)(\var) \\
        & = \tctx_0(\var) +_{i=1}^{n} \tctx_i(\var) \\
        & = \set{\typ_{0,0},\hdots,\typ_{0,m_0}} +_{i=1}^{n} \set{\typ_{i,0},\hdots,\typ_{i,m_i}} \\
        & = \set{\typ_{0,0},\hdots,\typ_{0,m_0}, \hdots, \typ_{n,0},\hdots,\typ_{n,m_n}}\\
    \end{split}\end{equation*}
\end{enumerate}
\end{proof}
